src/Verifier/SpecConversions.dfy
@@ -15,7 +15,7 @@ module SpecConversions {
 
   function ToCheck(spec: seq<AExpr>): (stmts: seq<Stmt>)
     requires AstValid.AExprSeq(spec)
-    ensures AstValid.StmtSeq(stmts) && JustPredicateStmts(stmts)
+    ensures AstValid.StmtSeq(stmts) && JustPredicateStmts(stmts) && |spec| == |stmts|
   {
     if spec == [] then
       []
@@ -32,7 +32,7 @@ module SpecConversions {
 
   function ToLearn(spec: seq<AExpr>): (stmts: seq<Stmt>)
     requires AstValid.AExprSeq(spec)
-    ensures AstValid.StmtSeq(stmts) && JustPredicateStmts(stmts)
+    ensures AstValid.StmtSeq(stmts) && JustPredicateStmts(stmts) && |spec| == |stmts|
   {
     if spec == [] then
       []
